\documentclass{article}

\usepackage[letterpaper, portrait, margin=0.8in]{geometry}

\usepackage{amsmath, amsfonts, amsthm, amssymb}
\usepackage{graphicx, float}
\usepackage{mathtools}
\usepackage{siunitx}
\usepackage{esdiff}
\usepackage{titlesec}
\usepackage{hyperref}

%opening
\title{PCH Winter Summary}
\author{Jayden Li}
\date{December 2023 -- February 2024}

\begin{document}

\maketitle

\linespread{1.25}
\fontsize{12pt}{12pt}\selectfont

\section{Trigonometry}
\subsection{Pythagorean Identity}
\begin{center}
	$\sin^2x+\cos^2x=1$
\end{center}

\subsection{Even/Odd Identities}
\begin{center}
	Cosine is even. $\cos\left(-\theta\right)=\cos\theta$ \\
	Sine is odd. $\sin\left(-\theta\right)=-\sin\theta$ \\
	Tangent is odd. $\tan\left(-\theta\right)=-\tan\theta$ \\
\end{center}

\subsection{Angle Addition and Subtraction Identities}
\begin{gather*}
	\sin\left(\alpha+\beta\right)=
	\sin\alpha\cos\beta+\cos\alpha\sin\beta \\
	\sin\left(\alpha-\beta\right)=
	\sin\alpha\cos\beta-\cos\alpha\sin\beta \\
	\cos\left(\alpha+\beta\right)=
	\cos\alpha\cos\beta-\sin\alpha\sin\beta \\
	\cos\left(\alpha-\beta\right)=
	\cos\alpha\cos\beta+\sin\alpha\sin\beta \\
	\hyperref[proof:tanadd]{
		\tan\left(\alpha+\beta\right)=
		\frac{\tan\alpha+\tan\beta}{1-\tan\alpha\tan\beta}
		} \\
	\hyperref[proof:tansub]{
		\tan\left(\alpha-\beta\right)=
		\frac{\tan\alpha-\tan\beta}{1+\tan\alpha\tan\beta}
	} \\
\end{gather*}

\subsection{Double Angle Identites}
\begin{gather*}
	\hyperref[proof:sindouble]{
		\sin2\theta=2\sin\theta\cos\theta
	} \\
	\hyperref[proof:cosdouble]{
		\begin{aligned}
			\cos2\theta&=\cos^2\theta-\sin^2\theta \\
			&=1-2\sin^2\theta \\
			&=2\cos^2\theta-1 \\
		\end{aligned}
	} \\
	\hyperref[proof:tandouble]{
		\tan2\theta=\frac{2\tan\theta}{1-\tan^2\theta}
	} \\
\end{gather*}

\subsection{Product-to-Sum Identities}
\begin{center}
\hyperref[proof:p2s]{
	$\begin{aligned}
		\sin\alpha\cos\beta=\frac{\sin\left(\alpha+\beta\right)
			+\sin\left(\alpha-\beta\right)}{2} \\
		\cos\alpha\sin\beta=\frac{\sin\left(\alpha+\beta\right)
			-\sin\left(\alpha-\beta\right)}{2} \\
			\cos\alpha\cos\beta=\frac{\cos\left(\alpha-\beta\right)
				+\cos\left(\alpha+\beta\right)}{2} \\
		\sin\alpha\sin\beta=\frac{\cos\left(\alpha-\beta\right)
			-\cos\left(\alpha+\beta\right)}{2} \\
	\end{aligned}$
}
\end{center}







\pagebreak
\section{Derivations}

\subsection{Tangent Angle Addition}
\label{proof:tanadd}
\begin{proof}
	$\begin{aligned}[t]
		\tan\left(\alpha+\beta\right)
		&=\frac{\sin\left(\alpha+\beta\right)}
			 {\cos\left(\alpha+\beta\right)} \\
		&=\frac{\sin\alpha\cos\beta+\cos\alpha\sin\beta}
			 {\cos\alpha\cos\beta-\sin\alpha\sin\beta} \\
		&=\frac{\sin\alpha\cos\beta+\cos\alpha\sin\beta}{\cos\alpha\cos\beta}/
		\frac{\cos\alpha\cos\beta-\sin\alpha\sin\beta}{\cos\alpha\cos\beta} \\
		&=\left(\frac{\sin\alpha\cos\beta}{\cos\alpha\cos\beta}+
		\frac{\cos\alpha\sin\beta}{\cos\alpha\cos\beta}\right)/
		\left(\frac{\cos\alpha\cos\beta}{\cos\alpha\cos\beta}-
		\frac{\sin\alpha\sin\beta}{\cos\alpha\cos\beta}\right) \\
		&=\boxed{\frac{\tan\alpha+\tan\beta}{1-\tan\alpha\tan\beta}} \\
	\end{aligned} \\$
\end{proof}

\subsection{Tangent Angle Subtraction}
\label{proof:tansub}
\begin{proof}
	$\begin{aligned}[t]
		\tan\left(\alpha-\beta\right)
		&=\tan\left(\alpha+\left(-\beta\right)\right) \\
		&=\frac{\tan\alpha+\tan\left(-\beta\right)}
			 {1-\tan\alpha\tan\left(-\beta\right)} \\
		&=\frac{\tan\alpha+\left(-\tan\beta\right)}
			 {1-\tan\alpha\cdot\left(-\tan\beta\right)} \\
		&=\boxed{\frac{\tan\alpha-\tan\beta}{1+\tan\alpha\tan\beta}} \\
	\end{aligned} \\$
\end{proof}

\subsection{Sine Double Angle}
\label{proof:sindouble}
\begin{proof}
	$\begin{aligned}[t]
		\sin2\theta&=\sin\left(\theta+\theta\right) \\
		&=\sin\theta\cos\theta+\cos\theta\sin\theta \\
		&=\boxed{2\sin\theta\cos\theta} \\
	\end{aligned} \\$
\end{proof}

\subsection{Cosine Double Angle}
\label{proof:cosdouble}
\begin{proof}
	$\begin{aligned}[t]
		\cos2\theta&=\cos\left(\theta+\theta\right) \\
		&=\cos\theta\cos\theta-\sin\theta\sin\theta \\
		&=\boxed{\cos^2\theta-\sin^2\theta} \\
		&=\cos^2\theta-\left(1-\cos^2\theta\right) \\
		&=\boxed{2\cos^2\theta-1} \\
		&=2\left(1-\sin^2\theta\right)-1 \\
		&=\boxed{1-2\sin^2\theta} \\
	\end{aligned} \\$
\end{proof}

\subsection{Tangent Double Angle}
\label{proof:tandouble}
\begin{proof}
	$\begin{aligned}[t]
		\tan2\theta&=\tan\left(\theta+\theta\right) \\
		&=\frac{\tan\theta+\tan\theta}{1-\tan\theta\tan\theta} \\
		&=\boxed{\frac{2\tan\theta}{1-\tan^2\theta}} \\
	\end{aligned} \\$
\end{proof}

\subsection{Product-to-Sum Identities}
\label{proof:p2s}
\begin{proof}
	\begin{align}
		\sin\left(\alpha+\beta\right)=
		\sin\alpha\cos\beta+\cos\alpha\sin\beta \\
		\sin\left(\alpha-\beta\right)=
		\sin\alpha\cos\beta-\cos\alpha\sin\beta \\
		\cos\left(\alpha+\beta\right)=
		\cos\alpha\cos\beta-\sin\alpha\sin\beta \\
		\cos\left(\alpha-\beta\right)=
		\cos\alpha\cos\beta+\sin\alpha\sin\beta
	\end{align}
	\begin{align*}
		\intertext{\centering{$(1)+(2)$}}
		\sin\left(\alpha+\beta\right)+\sin\left(\alpha-\beta\right)&=
		\sin\alpha\cos\beta+\cos\alpha\sin\beta
		+\sin\alpha\cos\beta-\cos\alpha\sin\beta \\
		\sin\left(\alpha+\beta\right)+\sin\left(\alpha-\beta\right)&=
		2\sin\alpha\cos\beta \\
		\Aboxed{\sin\alpha\cos\beta&=\frac{\sin\left(\alpha+\beta\right)
		+\sin\left(\alpha-\beta\right)}{2}}
	\end{align*}
	\begin{align*}
		\intertext{\centering{$(1)-(2)$}}
		\sin\left(\alpha+\beta\right)-\sin\left(\alpha-\beta\right)&=
		\sin\alpha\cos\beta+\cos\alpha\sin\beta
		-\sin\alpha\cos\beta+\cos\alpha\sin\beta \\
		\sin\left(\alpha+\beta\right)-\sin\left(\alpha-\beta\right)&=
		2\cos\alpha\sin\beta \\
		\Aboxed{\cos\alpha\sin\beta&=\frac{\sin\left(\alpha+\beta\right)
		-\sin\left(\alpha-\beta\right)}{2}}
	\end{align*}
	\begin{align*}
		\intertext{\centering{$(3)+(4)$}}
		\cos\left(\alpha+\beta\right)+\cos\left(\alpha-\beta\right)&=
		\cos\alpha\cos\beta-\sin\alpha\sin\beta
		+\cos\alpha\cos\beta+\sin\alpha\sin\beta \\
		\cos\left(\alpha+\beta\right)+\cos\left(\alpha-\beta\right)&=
		2\cos\alpha\cos\beta \\
		\Aboxed{\cos\alpha\cos\beta&=\frac{\cos\left(\alpha-\beta\right)
		+\cos\left(\alpha+\beta\right)}{2}}
	\end{align*}
	\begin{align*}
		\intertext{\centering{$(3)-(4)$}}
		\cos\left(\alpha+\beta\right)-\cos\left(\alpha-\beta\right)&=
		\cos\alpha\cos\beta-\sin\alpha\sin\beta
		-\cos\alpha\cos\beta-\sin\alpha\sin\beta \\
		\cos\left(\alpha+\beta\right)-\cos\left(\alpha-\beta\right)&=
		-2\sin\alpha\sin\beta \\
		\sin\alpha\sin\beta&=-\frac{\cos\left(\alpha+\beta\right)
		-\cos\left(\alpha-\beta\right)}{2} \\
		\Aboxed{\sin\alpha\sin\beta&=\frac{\cos\left(\alpha-\beta\right)
		-\cos\left(\alpha+\beta\right)}{2}}
	\end{align*}
\end{proof}


\end{document}
